src/program_logic/simulation.v
@@ -1,0 +1,36 @@
+From Perennial.Helpers Require Import Transitions.
+From iris.base_logic Require Import base_logic lib.invariants.
+From iris.proofmode Require Import tactics.
+From iris_string_ident Require Import ltac2_string_ident.
+From iris.prelude Require Import options.
+
+Section simulation.
+  Context `{!invG Σ}.
+  Context {state: Type} (wf: state -> Prop) (P: state -> iProp Σ).
+  Context (E: coPset).
+  (* TODO: if we can start using this everywhere I think we can start proving
+  generic theorems about simulation, like the one below *)
+  Definition simulation_fupd {T} (tr: transition state T) (Q: T -> iProp Σ): iProp Σ :=
+    (∀ σ σ' r,
+         ⌜wf σ⌝ -∗
+         ⌜relation.denote tr σ σ' r⌝ -∗
+        (P σ ={E}=∗ P σ' ∗ ⌜wf σ'⌝ ∗ Q r)).
+
+  Theorem simulation_bind_fupd {A B}
+          (tr1: transition state A)
+          (tr2: A -> transition state B)
+          (Q: B -> iProp Σ) :
+    simulation_fupd tr1 (fun x => simulation_fupd (tr2 x) Q) -∗
+    simulation_fupd (bind tr1 tr2) Q.
+  Proof.
+    iIntros "Hfupd".
+    iIntros (σ1 σ3 r Hwf Htr) "HP".
+    simpl in Htr.
+    inversion Htr; subst; clear Htr.
+    rename s2 into σ2.
+    iMod ("Hfupd" with "[] [] HP") as "(HP&%Hwf2&Hfupd2)"; eauto.
+    iMod ("Hfupd2" with "[] [] HP") as "(HP&%Hwf3&HQ)"; eauto.
+    iFrame.
+    auto.
+  Qed.
+End simulation.
