src/program_proof/wal/sliding.v
@@ -216,3 +216,41 @@ Proof.
     rewrite !apply_upds_insert_commute; auto.
     rewrite insert_insert //.
 Qed.
+
+Lemma memWrite_one_NoDup σ u :
+  NoDup (update.addr <$> σ.(slidingM.log)) →
+  int.Z σ.(slidingM.mutable) - int.Z σ.(slidingM.start) = 0 →
+  NoDup (update.addr <$> (memWrite_one σ u).(slidingM.log)).
+Proof.
+  intros Hnodup Hro_len.
+  rewrite /memWrite_one.
+  destruct (find_highest_index _) as [i|] eqn:Hlookup; simpl.
+  - rewrite Hro_len.
+    rewrite -> decide_True by word.
+    simpl.
+    rewrite list_fmap_insert.
+    rewrite list_insert_id //.
+    apply find_highest_index_ok' in Hlookup as [Hlookup _].
+    auto.
+  - rewrite fmap_app.
+    apply NoDup_app.
+    split_and!; auto.
+    + simpl.
+      intros x Hx ->%elem_of_list_singleton.
+      apply elem_of_list_lookup in Hx as [txn_id Hx].
+      eapply find_highest_index_none in Hlookup; eauto.
+    + simpl.
+      apply NoDup_singleton.
+Qed.
+
+Lemma memWrite_all_NoDup σ bufs:
+  NoDup (update.addr <$> σ.(slidingM.log)) →
+  int.Z σ.(slidingM.mutable) - int.Z σ.(slidingM.start) = 0 →
+  NoDup (update.addr <$> (memWrite σ bufs).(slidingM.log)).
+Proof.
+  generalize dependent σ.
+  induction bufs as [|u bufs]; simpl; intuition.
+  apply IHbufs.
+  - apply memWrite_one_NoDup; auto.
+  - rewrite memWrite_one_same_start memWrite_one_same_mutable //.
+Qed.
